code/experimental/P256/Hacl.Impl.P256.fsti
@@ -138,12 +138,6 @@ val norm: p: point -> resultPoint: point -> tempBuffer: lbuffer uint64 (size 32)
   )
 
 
-val montgomery_ladder: p: point -> q: point ->
-  scalarSize: size_t -> scalar: lbuffer uint8 scalarSize -> 
-  tempBuffer:  lbuffer uint64 (size 100)  -> 
-  Stack unit
-  (requires fun h -> live h p /\ live h tempBuffer)
-  (ensures fun h0 _ h1 -> True)
 
 val scalarMultiplication: p: point -> result: point -> 
   scalar: lbuffer uint8 (size 32) -> 
